Logic/DL/Syntax.lean
@@ -7,12 +7,14 @@ inductive Relation (RelType: Type) : Type
   | comp : Relation RelType → Relation RelType → Relation RelType -- composition α.β
   | alt : Relation RelType → Relation RelType → Relation RelType -- alternation α ∪ β
   | iter : Relation RelType → Relation RelType --iteration α*
+deriving DecidableEq, BEq
 
 inductive DLForm (RelType AtomType: Type) : Type
   | atom : AtomType → DLForm RelType AtomType -- atomic propositions modelled as strings
   | falsum : DLForm RelType AtomType -- falsum ⊥
   | imp : DLForm RelType AtomType → DLForm RelType AtomType → DLForm RelType AtomType -- implication φ → ψ
   | diamond : Relation RelType → DLForm RelType AtomType → DLForm RelType AtomType -- diamond ⟨α⟩φ
+deriving DecidableEq, BEq
 
 --derived syntactic sugar
 open DLForm
