Logic/Tableau/Proofs.lean
@@ -1,0 +1,16 @@
+import Logic.Tableau.Tableau
+import Logic.REPEAT.Semantics
+
+open Logic.DL
+
+
+def SatisfiesBranch (E: LiberalExecution) (branch: Branch) : Prop :=
+  sorry
+
+
+-- given a branch is satisfied by E, then at least one rule generated branch is satisfied
+def RuleSound (r: Rule) : Prop :=
+  ∀ E sel branches,
+    SatisfiesBranch E sel.branch ∧
+    r sel = some branches →
+      ∃ b ∈ branches, SatisfiesBranch E b
