Logic/Tableau/Tableau.lean
@@ -1,0 +1,224 @@
+import Logic.REPEAT.Syntax
+import Logic.DL.Syntax
+import Logic.Common.DynamicIndex
+
+namespace Logic.DL
+
+abbrev FreeVar := String
+
+-- at verification/tableau level, also @fn, evaluating to the proc id is an expression
+inductive TExpr : Type
+  | program : Expr → TExpr
+  | fn : TExpr
+deriving DecidableEq, BEq
+
+
+inductive TCond : Type
+  | le : TExpr → TExpr → TCond
+deriving DecidableEq, BEq
+
+-- temporary new DAForm to include @fn
+abbrev TDAForm := DLForm DynIndex TCond
+
+
+inductive Sign : Type
+  | pos : Sign
+  | neg : Sign
+deriving DecidableEq, BEq
+
+-- represents an indexed formula s: φ as {Sign.pos, s, φ} or s̄: φ as {Sign.neg, s, φ}
+structure IndexedForm where
+  sign : Sign
+  index: DynIndex
+  form : TDAForm
+deriving DecidableEq, BEq
+
+-- represents an indexed expr x = s: ⌞e⌟ as {x, s, e}
+structure IndexedExpr where
+  free_var : FreeVar
+  index : DynIndex
+  expr : TExpr
+deriving DecidableEq, BEq
+
+-- represents an indexed program variable x = s: a[y] as {x, s, a, y}
+structure IndexedVar where
+  free_var : FreeVar
+  index : DynIndex
+  arr : Var
+  arr_idx : FreeVar
+deriving DecidableEq, BEq
+
+-- type representing the arithmetic expression over free variables in tableau nodes
+inductive AExp: Type
+  | var : FreeVar → AExp
+  | const : Int → AExp
+  | add : AExp → AExp → AExp
+  | neg : AExp → AExp
+deriving DecidableEq, BEq
+
+-- arithmetic constraints (i.e. e₁ ≤ e₂ or e₁ = e₂)
+inductive ArithConstraint: Type
+  | le : AExp → AExp → ArithConstraint
+  | eq : AExp → AExp → ArithConstraint
+deriving DecidableEq, BEq
+
+-- representing a tableau node, being either an indexed formula, expression, program variable or arithmetic constraint
+inductive TableauNode: Type
+  | form  : IndexedForm → TableauNode
+  | expr  : IndexedExpr → TableauNode
+  | var   : IndexedVar → TableauNode
+  | arith : ArithConstraint → TableauNode
+deriving DecidableEq, BEq
+
+-- a branch is a list of tableau nodes
+abbrev Branch := List TableauNode
+
+-- stores the rule target nodes, i.e. the nodes a rule is applied on
+structure Selection where
+  branch : Branch
+  positions : List (Fin branch.length)
+
+def Selection.nodes (sel: Selection) : List TableauNode :=
+  sel.positions.map sel.branch.get
+
+-- given a selection of nodes, a rule application generates a list of branches if applicable.
+abbrev Rule := Selection → Option (List Branch)
+
+
+/- # Rule definitions -/
+
+def suitableVar (branch: Branch) (s: DynIndex) (e: TExpr) : FreeVar :=
+  sorry
+
+/-  s: φ → ψ
+(→)-------------
+    s̄: φ | s: ψ
+-/
+def posImpRule : Rule :=
+  λ sel ↦
+    match sel.nodes with
+    | [TableauNode.form               -- selected node is s: φ → ψ
+       {sign := Sign.pos,
+        index := s,
+        form := DLForm.imp φ ψ
+      }] =>
+        some [
+          --first branch
+          sel.branch ++ [
+            TableauNode.form {        -- append node s̄: φ
+              sign := Sign.neg,
+              index := s
+              form := φ
+            }],
+          --second branch
+          sel.branch ++ [
+            TableauNode.form {        -- append node s: ψ
+              sign := Sign.pos,
+              index := s
+              form := ψ
+            }
+          ]
+        ]
+    | _ => none                       -- return none iff rule is not applicable wrt selection
+
+
+/-  s̄: φ → ψ
+(̄→)----------
+    s: φ
+    s̄: ψ
+-/
+def negImpRule : Rule :=
+  λ sel ↦
+    match sel.nodes with
+    | [TableauNode.form               -- selected node is s̄: φ → ψ
+       {sign := Sign.neg,
+        index := s,
+        form := DLForm.imp φ ψ
+      }] =>
+        some [
+          sel.branch ++ [
+            TableauNode.form {        -- append node s: φ
+              sign := Sign.pos,
+              index := s,
+              form := φ
+            },
+            TableauNode.form {        -- append node s̄: ψ
+              sign := Sign.neg,
+              index := s,
+              form := ψ
+            }
+          ]
+        ]
+    | _ => none                       -- return none iff rule is not applicable wrt selection
+
+/-
+    s: ⊥
+(⊥)-------
+      ×
+-/
+def posFalsumRule : Rule :=
+  λ sel ↦
+    match sel.nodes with
+    | [TableauNode.form
+       {sign := Sign.pos,
+        index := _,
+        form := DLForm.falsum
+      }] => some []                   -- close branch, i.e. return empty list []
+    | _ => none
+
+/-
+    ̄s: ⊥
+(̄→)------
+
+-/
+def negFalsumRule : Rule :=
+  λ sel ↦
+    match sel.nodes with
+    | [TableauNode.form
+       {sign := Sign.neg,
+        index := _,
+        form := DLForm.falsum
+      }] => some [sel.branch]         -- return unmodified branch (no-op)
+    | _ => none
+
+/-
+    s: ⌞e₁ ≤ e₂⌟
+(≤)-------------- x, y suitable
+       x ≤ y
+     x = s:⌞e₁⌟
+     y = s:⌞e₂⌟
+-/
+def posLeRule : Rule :=
+  λ sel ↦
+    match sel.nodes with
+    | [TableauNode.form
+       {sign := Sign.pos,
+        index := s,
+        form := DLForm.atom (TCond.le e₁ e₂)}] =>
+
+          let x := suitableVar sel.branch s e₁
+          let y := suitableVar sel.branch s e₂
+
+          some [
+            sel.branch ++ [
+              -- append node x ≤ y
+              TableauNode.arith (ArithConstraint.le (AExp.var x) (AExp.var y)),
+
+              -- append node x = s:⌞e₁⌟
+              TableauNode.expr {
+                free_var := x,
+                index := s,
+                expr := e₁
+              },
+              -- append node y = s:⌞e₂⌟
+              TableauNode.expr {
+                free_var := y,
+                index := s,
+                expr := e₂
+              }
+            ]
+
+          ]
+    | _ => none
+
+end Logic.DL
